theories/graphsem.v
@@ -9,32 +9,41 @@ Unset Printing Implicit Defensive.
 From mathcomp Require Import order eqtype fintype finset seq choice ssrnat.
 (* Import Order.LTheory. *)
 
+From Coq Require Import Sets.Ensembles.
+
 From Lagois Require Import lagoisgraph.
 (* Open Scope order_scope. *)
 (* From Coq Require Import Logic.EqdepFacts. *)
 (* Require Import Coq.Arith.Wf_nat. *)
 
+
 Definition Var := nat.
 Definition Ch := nat.
 Definition Val := nat.
 
-Definition Env := Var -> Val.
-
+(* Abstract syntax of expressions *)
 Inductive Exp : Set :=
   | const : Val -> Exp
   | var : Var -> Exp
   | add : Exp -> Exp -> Exp
-  | not : Exp -> Exp.
+  | sub : Exp -> Exp -> Exp
+  | not : Exp -> Exp
+  | cmp : Exp -> Exp -> Exp.
 
-Fixpoint ExpSem (m : Env) (e : Exp)  : Val :=
+(* Definition of m(e) *)
+Definition Mem := Var -> Val.
+Fixpoint ExpSem (m : Mem) (e : Exp)  : Val :=
   match e with
   | const n => n
   | var v => m v
   | add e1 e2 => ExpSem m e1 + ExpSem m e2
+  | sub e1 e2 => ExpSem m e1 - ExpSem m e2
   | not e' => if 0 < ExpSem m e' then 0 else 1
+  | cmp e1 e2 => ExpSem m e1 == ExpSem m e2
   end.
 
-Inductive Stmt : Type :=
+(* Abstract syntax of statements *)
+Inductive Stmt : Set :=
   | skip : Stmt
   | assign : Var -> Exp -> Stmt
   | output : Ch -> Exp -> Stmt
@@ -43,64 +52,153 @@ Inductive Stmt : Type :=
   | while : Exp -> Stmt -> Stmt
   | seque : Stmt -> Stmt -> Stmt.
 
-Inductive Event {G : LagoisGraph.type} : Type :=
-  | ε_ev : Event
-  | update  : G -> Var -> Val -> Event.
+Definition State := (Stmt * Mem)%type.
 
-Definition State := prod Stmt Env.
+(* Definition of signals *)
+Inductive Sig : Type :=
+  | ε_sig : Sig
+  | ass_sig : Var -> Sig
+  | out_sig : Ch -> Val -> Sig
+  | in_sig : Ch -> Var -> Val -> Sig.
+
+(* Small steps semantics of local execution *)
+Inductive SemSS : State -> Sig -> State -> Prop :=
+  | ex_assign m x e n :
+      ExpSem m e = n ->
+      SemSS (assign x e, m) (ass_sig x)
+          (skip, fun_of_simpl [eta m with x |-> n])
+  | ex_out m c e n:
+      ExpSem m e = n ->
+      SemSS (output c e, m) (out_sig c n) (skip, m)
+  | ex_in m c x n :
+      SemSS (input c x, m) (in_sig c x n)
+          (skip, fun_of_simpl [eta m with x |-> n])
+  | ex_ifelse_ff e s1 s2 m :
+      ExpSem m e = 0 ->
+      SemSS (ifelse e s1 s2, m) ε_sig (s2, m)
+  | ex_ifelse_tt e s1 s2 m :
+      0 < ExpSem m e ->
+      SemSS (ifelse e s1 s2, m) ε_sig (s1, m)
+  | ex_while e s m :
+      SemSS (while e s, m) ε_sig (ifelse e (seque s (while e s)) skip, m)
+  | ex_seque_cont s1 s1' s2 m m' ϕ :
+      SemSS (s1, m) ϕ (s1', m') ->
+      SemSS (seque s1 s2, m) ϕ (seque s1' s2, m')
+  | ex_seque_skip s m :
+      SemSS (seque skip s, m) ε_sig (s, m).
+
+(* Definition of events *)
+Inductive Ev G : Type :=
+  | ε_ev : Ev G
+  | ass_ev : G -> Var -> Ev G.
+Arguments ε_ev {G}.
 
 Definition GState (G : LagoisGraph.type) := G -> State.
 
-Inductive GSemSS G : GState G -> Event -> GState G -> Prop :=
-  | ex_assign (Gst : GState G) v m i e :
-      Gst v = (assign i e, m) ->
-      GSemSS Gst (update v i (ExpSem m e)) [eta Gst with v |-> (skip, fun_of_simpl [eta m with i |-> (ExpSem m e)])]
-  | ex_exch (Gst : GState G) v m v' m' c i' e :
-      Gst v = (output c e, m) ->
-      Gst v' = (input i' c, m') ->
-      GSemSS Gst (update v' i' (ExpSem m e)) [eta Gst with v  |-> (skip, m),
-                                                           v' |-> (skip, fun_of_simpl [eta m' with i' |-> (ExpSem m e)])]
-  | ex_ifelse_ff (Gst : GState G) v b s1 s2 m :
-      Gst v = (ifelse b s1 s2, m) ->
-      ExpSem m b = 0 ->
-      GSemSS Gst ε_ev [eta Gst with v |-> (s2, m)]
-  | ex_ifelse_tt (Gst : GState G) v b s1 s2 m :
-      Gst v = (ifelse b s1 s2, m) ->
-      ExpSem m b > 0 ->
-      GSemSS Gst ε_ev [eta Gst with v |-> (s1, m)]
-  | ex_while (Gst : GState G) v b s m :
-      Gst v = (while b s, m) ->
-      ExpSem m b = 0 ->
-      GSemSS Gst ε_ev [eta Gst with v |-> (ifelse b (seque s (while b s)) skip, m)]
-  | ex_seque_cont (Gst Gst': GState G) v s1 s1' s2 m m' ev :
-      Gst v = (seque s1 s2, m) ->
-      GSemSS [eta Gst with v |-> (s1, m)] ev Gst' ->
-      Gst' v = (s1', m') ->
-      GSemSS Gst ev [eta Gst with v |-> (seque s1' s2, m')]
-  | ex_seque_skip (Gst Gst': GState G) v s m :
-      Gst v = (seque skip s, m) ->
-      GSemSS Gst ε_ev [eta Gst with v |-> (s, m)].
+(* Small steps semantics of distributed execution *)
+Inductive GSemSS G : GState G -> Ev G -> GState G -> Prop :=
+  | ex_sp St v st st':
+      St v = st ->
+      SemSS st ε_sig st' ->
+      GSemSS St ε_ev [eta St with v |-> st']
+  | ex_lp St v st st' x :
+      St v = st ->
+      SemSS st (ass_sig x) st' ->
+      GSemSS St (ass_ev v x) [eta St with v |-> st']
+  | ex_exch St v_i v_j f st_i st'_i st_j st'_j c x n:
+      v_i @f> v_j ->
+      St v_i = st_i ->
+      St v_j = st_j ->
+      SemSS st_i (out_sig c n) st'_i ->
+      SemSS st_j (in_sig c x n) st'_j ->
+      GSemSS St (ass_ev v_j x) [eta St with v_i |-> st'_i, v_j |-> st'_j].
 
-Inductive GSemBS G : GState G -> seq Event -> GState G -> Type :=
-  | sem_refl (Gst  : GState G) : GSemBS Gst [::] Gst
-  | sem_trans (Gst Gst' Gst'' : GState G) evs ev :
-      GSemBS Gst evs Gst' ->
-      GSemSS Gst' ev Gst'' ->
-      GSemBS Gst (ev :: evs) Gst''.
+(* Definition 17 *)
+Inductive Trace G : GState G -> GState G -> Type :=
+  | exs_refl St : Trace St St
+  | exs_trans St St' St'' α :
+      Trace St St' ->
+      GSemSS St' α St'' ->
+      Trace St St''.
 
-Record Atk (G : LagoisGraph.type) (loc : G) (lvl : L(loc)) := {
-  Sts : Type;
-  init : Sts;
-  tfun : @Event G -> Sts -> Sts;
+Definition PMem := (Var -> option Val).
+
+(* Definition 18 *)
+HB.mixin Record IsAtk (G : LagoisGraph.type) Σ := {
+  σ_init : Σ;
+  δ : Σ -> PMem -> Σ;
 }.
+HB.structure Definition Atk G := {Sts of IsAtk G Sts}.
 
-Fixpoint observe (G : LagoisGraph.type) (loc : G) (sec : Var -> L(loc)) (lvl : L(loc)) (a : Atk lvl) (Gst Gst' : GState G) evs (trace : GSemBS Gst evs Gst') : Sts a :=
-  match trace with
-  | sem_refl Gst0  => init a
-  | sem_trans _ _ _ _ ev trace' _ =>
-      let st := observe sec a trace' in match ev with
-                                    | ε_ev => st
-                                    | update v i n => if v == loc && sec i <= lvl then
-                                    end
+Section Security.
 
+Variables (G : LagoisGraph.type)
+    (A : Atk.type G) (loc : G) (lvl : L(loc)) (λ : Var -> L(loc)).
+
+(* Definition of observable sequences *)
+Definition obs (m : Mem) : PMem :=
+  fun x => if (λ x <= lvl) then Some (m x) else None.
+
+Fixpoint Obs St St'' (t : @Trace G St St'') : seq PMem :=
+  match t with
+  | exs_refl St => [:: obs (St loc).2]
+  | exs_trans St St' St'' α t' _ =>
+      let μs := Obs t' in
+        match α with
+        | ε_ev => μs
+        | ass_ev v x => if (loc == v) && (λ x <= lvl)
+                       then obs (St'' loc).2 :: μs
+                       else μs
+        end
   end.
+
+(* Definition of State emitting observable sequence *)
+Definition GSemTrace (St : GState G) (μs : seq PMem) : Prop :=
+  exists St' (t : Trace St St'), Obs t = μs.
+
+(* Definition of A(μs) *)
+Fixpoint observe (μs : seq PMem) : A :=
+  match μs with
+  | [::] => σ_init
+  | μ :: μs' => δ (observe μs') μ
+  end.
+
+(* Definition of knowledge *)
+Definition k (S : G -> Stmt) (σ : A) : Ensemble Mem :=
+  fun m => exists St μs, GSemTrace St μs
+                            /\ (forall v, (St v).1 = S v)
+                            /\ (St loc).2 = m
+                            /\ observe μs = σ.
+
+Definition k_plus (S : G -> Stmt) (σ : A) : Ensemble Mem :=
+  fun m => exists St μs μ, GSemTrace St (μ :: μs)
+                            /\ (forall v, (St v).1 = S v)
+                            /\ (St loc).2 = m
+                            /\ observe μs = σ.
+
+(* Definition of observable initial memory *)
+Definition m_equiv (m m' : Mem) : Prop :=
+  forall x, λ x <= lvl -> m x = m' x.
+
+Definition m_equiv_class (m : Mem) : Ensemble Mem :=
+  fun m' => m_equiv m m'.
+
+(* Definition 19 *)
+Definition nonintf (St : GState G) : Prop :=
+  forall μs μ, GSemTrace St (μ :: μs) ->
+    Included _
+      (Intersection _
+        (m_equiv_class (St loc).2)
+        (k (fun v => (St v).1) (observe μs)))
+      (k (fun v => (St v).1) (observe (μ :: μs))).
+
+(* Definition 20 *)
+Definition pi_nonintf (St : GState G) : Prop :=
+  forall μs μ, GSemTrace St (μ :: μs) ->
+    Included _
+      (Intersection _
+        (m_equiv_class (St loc).2)
+        (k_plus (fun v => (St v).1) (observe μs)))
+      (k (fun v => (St v).1) (observe (μ :: μs))).
+
+End Security.
