theories/sem.v
@@ -25,8 +25,9 @@ Definition eqVar x y :=
 Lemma eqVarP : Equality.axiom eqVar.
 Proof.
   rewrite/Equality.axiom => x y.
-  case x_eq_y: (eqVar x y); case: x x_eq_y => x; case: y => y //= x_eq_y; move/eqP in x_eq_y;
-    do 1? (apply: ReflectT; rewrite x_eq_y; by []);
+  case x_eq_y: (eqVar x y); case: x x_eq_y => x;
+  case: y => y //= x_eq_y; move/eqP in x_eq_y;
+  do 1? (apply: ReflectT; rewrite x_eq_y; by []);
   apply: ReflectF => //=; by rewrite/not in x_eq_y * => [[x_eq_y']].
 Qed.
 
@@ -42,7 +43,8 @@ HB.structure Definition BigStepSemantic T := {Term of isBigStepSemantic T Term}.
 
 Notation "s ==[ t ]==> s'" := (bigstep s t s') (at level 30).
 
-HB.mixin Record IsSubSemantic (Val Term : Type) of BigStepSemantic (Store Val) Term := {
+HB.mixin Record IsSubSemantic
+    (Val Term : Type) of BigStepSemantic (Store Val) Term := {
   determines : Term -> Var -> seq.seq Var ;
 
   assigned : Term -> Var -> bool ;
@@ -61,9 +63,11 @@ HB.mixin Record IsSubSemantic (Val Term : Type) of BigStepSemantic (Store Val) T
   xs_not_assigned : forall x t, ~~ (assigned t (exp x)) ;
   ys_not_assigned : forall y t, ~~ (assigned t (imp y)) ;
 }.
-HB.structure Definition SubSemantic Val := {Term of IsSubSemantic Val Term & BigStepSemantic Val Term}.
+HB.structure Definition SubSemantic Val :=
+  {Term of IsSubSemantic Val Term & BigStepSemantic Val Term}.
 
-Inductive commsem {Val : Type} {Term : SubSemantic.type Val} : Store Val -> command Term -> Store Val -> Prop :=
+Inductive commsem {Val : Type} {Term : SubSemantic.type Val} :
+    Store Val -> command Term -> Store Val -> Prop :=
   | Tsem μ ν t :
       μ ==[ t ]==> ν ->
       commsem μ (tsyn t) ν
@@ -71,9 +75,11 @@ Inductive commsem {Val : Type} {Term : SubSemantic.type Val} : Store Val -> comm
       commsem μ (wr x z) [eta μ with exp x |-> μ (loc  z)]
   | RDsem μ z y :
       commsem μ (rd z y) [eta μ with loc z |-> μ (imp y)].
-HB.instance Definition _ Val (Term : SubSemantic.type Val) := isBigStepSemantic.Build (Store Val) (command Term) commsem.
+HB.instance Definition _ Val (Term : SubSemantic.type Val) :=
+  isBigStepSemantic.Build (Store Val) (command Term) commsem.
 
-Inductive phrasesem {Val : Type} {Term Term' : SubSemantic.type Val} : Store2 Val -> phrase Term Term' -> Store2 Val -> Prop :=
+Inductive phrasesem {Val : Type} {Term Term' : SubSemantic.type Val} :
+    Store2 Val -> phrase Term Term' -> Store2 Val -> Prop :=
   | Lcommsem μ μ' ν c :
       μ ==[ c ]==> ν ->
       phrasesem (μ, μ') (csyn c) (ν, μ')
@@ -84,13 +90,16 @@ Inductive phrasesem {Val : Type} {Term Term' : SubSemantic.type Val} : Store2 Va
       phrasesem (μ, μ') (T_RL y x') ([eta μ with imp y |-> μ' (exp x')], μ')
   | TLRsem μ μ' y' x :
       phrasesem (μ, μ') (T_LR y' x) (μ, [eta μ' with imp y' |-> μ (exp x)]).
-HB.instance Definition _ Val (Term Term' : SubSemantic.type Val) := isBigStepSemantic.Build (Store2 Val) (phrase Term Term') phrasesem.
+HB.instance Definition _ Val (Term Term' : SubSemantic.type Val) :=
+  isBigStepSemantic.Build (Store2 Val) (phrase Term Term') phrasesem.
 
-Inductive seqsem {Val : Type} {Term Term': SubSemantic.type Val} : Store2 Val -> seq Term Term' -> Store2 Val -> Prop :=
+Inductive seqsem {Val : Type} {Term Term': SubSemantic.type Val} :
+    Store2 Val -> seq Term Term' -> Store2 Val -> Prop :=
   | εsem μ:
       seqsem μ ε μ
   | seqconssem s (p : phrase Term Term') μ μ1 μ2:
       seqsem μ s μ1 ->
       μ1 ==[ p ]==> μ2 ->
       seqsem μ (seqcons s p) μ2.
-HB.instance Definition _ Val (Term Term' : SubSemantic.type Val) := isBigStepSemantic.Build (Store2 Val) (seq Term Term') seqsem.
+HB.instance Definition _ Val (Term Term' : SubSemantic.type Val) :=
+  isBigStepSemantic.Build (Store2 Val) (seq Term Term') seqsem.
