theories/typrls.v
@@ -16,12 +16,13 @@ Section typrls.
 
 Variable Val : Type.
 Variable Term Term' : SubSemantic.type Val.
-Variable Q P : finTBLatticeType (Order.Disp tt tt).
-Variable f : { omorphism P -> Q}.
-Variable g : { omorphism Q -> P}.
-Variable HL : P<~f~g~>Q.
+Variable d d' : Order.disp_t.
+Variable P : finTBLatticeType d.
+Variable Q : finTBLatticeType d'.
+Variable fg : Lagois.type P Q.
 
-Inductive CommSType {A : finTBLatticeType (Order.Disp tt tt)} {Term0 : SubSemantic.type Val} : (Store A) -> command Term0 -> A -> Prop :=
+Inductive CommSType d {A : finTBLatticeType d} {Term0 : SubSemantic.type Val} :
+    (Store A) -> command Term0 -> A -> Prop :=
   | Tt (λ : Store A) t l:
       (forall z, assigned t z -> l <= λ z) ->
       (forall z, read t z -> λ z <= l) ->
@@ -33,7 +34,8 @@ Inductive CommSType {A : finTBLatticeType (Order.Disp tt tt)} {Term0 : SubSemant
       λ (loc z) <= λ (exp x) ->
       CommSType λ (wr x z) (λ (exp x)).
 
-Inductive PhraseSType : (Store P * Store Q) -> phrase Term Term' -> (P * Q) -> Prop :=
+Inductive PhraseSType :
+    (Store P * Store Q) -> phrase Term Term' -> (P * Q) -> Prop :=
   | LCT (λ : Store P) (λ' : Store Q) c l m':
       CommSType λ c l ->
       PhraseSType (λ, λ') (csyn c) (l, m')
@@ -41,10 +43,10 @@ Inductive PhraseSType : (Store P * Store Q) -> phrase Term Term' -> (P * Q) -> P
       CommSType λ' c' m' ->
       PhraseSType (λ, λ') (csyn' c') (l, m')
   | TTrl (λ : Store P) (λ' : Store Q) x' y :
-      g (λ' (exp x')) <= λ (imp y) ->
+      fg.2 (λ' (exp x')) <= λ (imp y) ->
       PhraseSType (λ, λ') (T_RL y x') (λ (imp y), λ' (exp x'))
   | TTlr (λ : Store P) (λ' : Store Q) x y' :
-      f (λ (exp x)) <= λ' (imp y') ->
+      fg.1 (λ (exp x)) <= λ' (imp y') ->
       PhraseSType (λ, λ') (T_LR y' x) (λ (exp x), λ' (imp y')).
 
 Inductive SeqSType : (Store P * Store Q) -> seq Term Term' -> (P * Q) -> Prop :=
@@ -55,7 +57,11 @@ Inductive SeqSType : (Store P * Store Q) -> seq Term Term' -> (P * Q) -> Prop :=
       SeqSType λ s t ->
       SeqSType λ (seqcons s p) (t_1.1 `&` t.1, t_1.2 `&` t.2).
 
-Lemma CommsSType_sound {A : finTBLatticeType (Order.Disp tt tt)} {Term0 : SubSemantic.type Val} (λ : Store A) τ τ_0 (μ ν μ' ν' : Store Val) (c : command Term0):
+Lemma CommsSType_sound
+    d0 (A : finTBLatticeType d0)
+    {Term0 : SubSemantic.type Val}
+    (λ : Store A) τ τ_0 (μ ν μ' ν' : Store Val)
+    (c : command Term0) :
   CommSType λ c τ_0 ->
   μ ==[ c ]==> μ' ->
   ν ==[ c ]==> ν' ->
@@ -63,14 +69,17 @@ Lemma CommsSType_sound {A : finTBLatticeType (Order.Disp tt tt)} {Term0 : SubSem
   (forall w : Var, λ w <= τ -> μ' w = ν' w).
 Proof.
   move=> λ_gives_c_type_τ' μ_c_μ' ν_c_ν' λw_le_τ_impl_μw_eq_νw w λw_le_τ.
-  have λw''_le_λw'_impl_μup_eq_νup : forall w' w'', λ w'' <= λ w' -> [eta μ with w' |-> μ w''] w = [eta ν with w' |-> ν w''] w.
+  have λw''_le_λw'_impl_μup_eq_νup :
+      forall w' w'', λ w'' <= λ w' ->
+          [eta μ with w' |-> μ w''] w = [eta ν with w' |-> ν w''] w.
     move=> w' w'' w'_le_w'' /=; case w_eq_expx: (w == w'); first last.
       exact: λw_le_τ_impl_μw_eq_νw λw_le_τ.
     apply: λw_le_τ_impl_μw_eq_νw.
     apply: (le_trans w'_le_w'').
     move/eqP: w_eq_expx => <-.
     exact: λw_le_τ.
-  inversion μ_c_μ'; subst; inversion ν_c_ν'; subst; inversion λ_gives_c_type_τ'; subst; first last.
+  inversion μ_c_μ'; subst; inversion ν_c_ν'; subst;
+      inversion λ_gives_c_type_τ'; subst; first last.
   - exact: λw''_le_λw'_impl_μup_eq_νup.
   - exact: λw''_le_λw'_impl_μup_eq_νup.
   - have w_notassin_t_impl_μ'w_eq_ν'w : ~~(assigned t w) -> μ' w = ν' w.
@@ -78,7 +87,8 @@ Proof.
       have <-: μ w = μ' w by apply: frame H w_notassin_t.
       have <-: ν w = ν' w by apply: frame H2 w_notassin_t.
       exact: λw_le_τ_impl_μw_eq_νw.
-    case: w λw_le_τ w_notassin_t_impl_μ'w_eq_ν'w {λw''_le_λw'_impl_μup_eq_νup} => n λn_le_τ w_notassin_t_impl_μ'w_eq_ν'w; first last.
+    case: w λw_le_τ w_notassin_t_impl_μ'w_eq_ν'w {λw''_le_λw'_impl_μup_eq_νup}
+        => n λn_le_τ w_notassin_t_impl_μ'w_eq_ν'w; first last.
     + exact: w_notassin_t_impl_μ'w_eq_ν'w (ys_not_assigned n t).
     + exact: w_notassin_t_impl_μ'w_eq_ν'w (xs_not_assigned n t).
     + case n_assin_t: (~~ (assigned t (loc n))).
@@ -93,31 +103,39 @@ Proof.
       exact: le_trans H4 τ0_le_τ.
 Qed.
 
-Lemma T_sound (A B : finTBLatticeType (Order.Disp tt tt)) (h : {omorphism A -> B}) (i : {omorphism B -> A}) (λ : Store A) (λ' : Store B) (m' : B) (y x' : ident) (w : Var) (μ ν μ' ν' : Store Val) :
-  A <~ h ~ i ~> B ->
-  m' = h (i m') ->
-  i (λ' (exp x')) <= λ (imp y) ->
-  λ w <= i m' ->
+Lemma T_sound
+    d0 (A : finTBLatticeType d0)
+    d0' (B : finTBLatticeType d0')
+    (hi : Lagois.type A B)
+    (λ : Store A) (λ' : Store B)
+    (m' : B) (y x' : ident)
+    (w : Var) (μ ν μ' ν' : Store Val) :
+  m' = hi.1 (hi.2 m') ->
+  hi.2 (λ' (exp x')) <= λ (imp y) ->
+  λ w <= hi.2 m' ->
   (forall w' : Var, λ' w' <= m' -> μ' w' =  ν' w') ->
-  (forall w : Var, λ w <= i m' -> μ w = ν w) ->
-  (if w == imp y then μ' (exp x') else μ w) = (if w == imp y then ν' (exp x') else ν w).
+  (forall w : Var, λ w <= hi.2 m' -> μ w = ν w) ->
+  (if w == imp y then μ' (exp x') else μ w) =
+      (if w == imp y then ν' (exp x') else ν w).
 Proof.
-  move=> LC m'_eq_him' iλ'x'_le_λy λw_le_im' μ'w'_eq_ν'w' μw_eq_νw.
+  move=> m'_eq_him' iλ'x'_le_λy λw_le_im' μ'w'_eq_ν'w' μw_eq_νw.
   case w_eq_y: (w == imp y); last first.
     exact: μw_eq_νw λw_le_im'.
   apply: μ'w'_eq_ν'w'.
-  have λ'x'_le_hiλ'x' : λ' (exp x') <= h (i (λ' (exp x')))
-    by move: LC => [LC1 _ _ _]; exact: LC1.
-  have iλ'x'_le_im' : i (λ' (exp x')) <= i m'
-    by move/eqP in w_eq_y; rewrite -w_eq_y in iλ'x'_le_λy; apply: le_trans iλ'x'_le_λy λw_le_im'.
-  have hiλ'x'_le_m' : h (i (λ' (exp x'))) <= m'.
-    by move/(omorph_le h) in iλ'x'_le_im'; rewrite -m'_eq_him' in  iλ'x'_le_im'.
+  have λ'x'_le_hiλ'x' : λ' (exp x') <= hi.1 (hi.2 (λ' (exp x')))
+    by exact: lc2.
+  have iλ'x'_le_im' : hi.2 (λ' (exp x')) <= hi.2 m'.
+    move/eqP in w_eq_y; rewrite -w_eq_y in iλ'x'_le_λy.
+    exact: le_trans iλ'x'_le_λy λw_le_im'.
+  have hiλ'x'_le_m' : hi.1 (hi.2 (λ' (exp x'))) <= m'.
+    move /(omorph_le hi.1) in iλ'x'_le_im'.
+    by rewrite -m'_eq_him' in  iλ'x'_le_im'.
   exact: le_trans λ'x'_le_hiλ'x' hiλ'x'_le_m'.
 Qed.
 
 Theorem SeqSType_sound l m' t_0 s λ μ μ_f ν ν_f :
-  l = g m' ->
-  m' = f l ->
+  l = fg.2 m' ->
+  m' = fg.1 l ->
   μ ==[ s ]==> μ_f ->
   ν ==[ s ]==> ν_f ->
   SeqSType λ s t_0 ->
@@ -128,24 +146,33 @@ Theorem SeqSType_sound l m' t_0 s λ μ μ_f ν ν_f :
 Proof.
   move=> l_eq_gm' m'_eq_fl μ_s_μf; elim: μ_s_μf ν ν_f t_0 λ.
     move=> {}μ ν ν_f t_0 λ ν_ε_νf; case ε_eq: _ _ / ν_ε_νf => //.
-  move=> s_1 p {}μ μ_1 {}μ_f μ_s1_μ1 IH μ1_p_μf ν ν_f t_0 λ ν_s1p_νf λ_gives_s1p_type_t0.
+  move=> s_1 p {}μ μ_1 {}μ_f μ_s1_μ1 IH μ1_p_μf ν ν_f t_0 λ
+         ν_s1p_νf λ_gives_s1p_type_t0.
   case E: _ _ / ν_s1p_νf => [|s_1' p' {}ν ν_1 {}ν_f ν_s1_ν1 ν1_p_νf]//.
-  move: E => [s1_eq_s1' p_eq_p']; rewrite -{s_1'}s1_eq_s1' in ν_s1_ν1; rewrite -{p'}p_eq_p' in ν1_p_νf.
-  case E: _ _ / λ_gives_s1p_type_t0 => [|{}λ t_p t_s p' s_1' λ_gives_p_tp λ_gives_s1_ts]//.
-  move: E => [s1_eq_s1' p_eq_p']; rewrite -{s_1'}s1_eq_s1' in λ_gives_s1_ts; rewrite -{p'}p_eq_p' in λ_gives_p_tp.
+  move: E => [s1_eq_s1' p_eq_p'].
+  rewrite -{s_1'}s1_eq_s1' in ν_s1_ν1; rewrite -{p'}p_eq_p' in ν1_p_νf.
+  case E: _ _ / λ_gives_s1p_type_t0 =>
+      [|{}λ t_p t_s p' s_1' λ_gives_p_tp λ_gives_s1_ts]//.
+  move: E => [s1_eq_s1' p_eq_p']; rewrite -{s_1'}s1_eq_s1' in λ_gives_s1_ts;
+      rewrite -{p'}p_eq_p' in λ_gives_p_tp.
   move=> μ1w_eq_ν1w μ2w_eq_ν2w.
-  move/(_ ν ν_1 t_s λ ν_s1_ν1 λ_gives_s1_ts μ1w_eq_ν1w μ2w_eq_ν2w): IH => {μ1w_eq_ν1w μ2w_eq_ν2w}[μ11w_eq_ν11w μ12w_eq_ν12w].
-  case: p μ1_p_μf ν1_p_νf λ_gives_p_tp => [ c | c' | y x' | y' x ] μ1_p_μf ν1_p_νf λ_gives_p_tp.
+  move/(_ ν ν_1 t_s λ ν_s1_ν1 λ_gives_s1_ts μ1w_eq_ν1w μ2w_eq_ν2w): IH =>
+      {μ1w_eq_ν1w μ2w_eq_ν2w}[μ11w_eq_ν11w μ12w_eq_ν12w].
+  case: p μ1_p_μf ν1_p_νf λ_gives_p_tp =>
+      [ c | c' | y x' | y' x ] μ1_p_μf ν1_p_νf λ_gives_p_tp.
   - inversion μ1_p_μf; inversion ν1_p_νf; inversion λ_gives_p_tp; subst.
     split => //; exact: CommsSType_sound H9 H1 H5 μ11w_eq_ν11w.
   - inversion μ1_p_μf; inversion ν1_p_νf; inversion λ_gives_p_tp; subst.
     split => //; exact: CommsSType_sound H9 H1 H5 μ12w_eq_ν12w.
   - inversion μ1_p_μf; inversion ν1_p_νf; inversion λ_gives_p_tp; subst => /=.
-    split=> [w λ0w_le_l | // ]; exact: T_sound HL m'_eq_fl H11 λ0w_le_l μ12w_eq_ν12w μ11w_eq_ν11w.
-  - inversion μ1_p_μf; inversion ν1_p_νf; inversion λ_gives_p_tp. move: l_eq_gm' m'_eq_fl. subst => l_eq_gm' m'_eq_fl /=.
+    split=> [w λ0w_le_l | // ].
+    exact: T_sound m'_eq_fl H11 λ0w_le_l μ12w_eq_ν12w μ11w_eq_ν11w.
+  - inversion μ1_p_μf; inversion ν1_p_νf; inversion λ_gives_p_tp.
+    move: l_eq_gm' m'_eq_fl. subst => l_eq_gm' m'_eq_fl /=.
     split=> [ // | w' λ'w_le_m'].
     rewrite m'_eq_fl in l_eq_gm' λ'w_le_m' μ12w_eq_ν12w.
-    exact: (T_sound (melton_3_2 HL) l_eq_gm' H11 λ'w_le_m' μ11w_eq_ν11w μ12w_eq_ν12w).
+    have l_eq_gm'_ : l = (fg.2, fg.1).1 ((fg.2, fg.1).2 l) by exact: l_eq_gm'.
+    exact (T_sound l_eq_gm'_ H11 λ'w_le_m' μ11w_eq_ν11w μ12w_eq_ν12w).
 Qed.
 
 End typrls.
